wip on updating decode_encode proof

src/Proofs/DecodeEncode.v
@@ -1,20 +1,21 @@
 Require Import Coq.ZArith.ZArith.
+Require Import Coq.Lists.List. Import ListNotations.
 Require Import riscv.Spec.Decode.
-Require Import riscv.Encode.
+Require Import riscv.Utility.Encode.
 Require Import riscv.Utility.Utility.
 Require Import riscv.Utility.Tactics.
 Require Import riscv.Utility.div_mod_to_quot_rem.
-Require Import riscv.proofs.invert_encode_R.
-Require Import riscv.proofs.invert_encode_R_atomic.
-Require Import riscv.proofs.invert_encode_I.
-Require Import riscv.proofs.invert_encode_I_shift_57.
-Require Import riscv.proofs.invert_encode_I_shift_66.
-Require Import riscv.proofs.invert_encode_I_system.
-Require Import riscv.proofs.invert_encode_S.
-Require Import riscv.proofs.invert_encode_SB.
-Require Import riscv.proofs.invert_encode_U.
-Require Import riscv.proofs.invert_encode_UJ.
-Require Import riscv.proofs.invert_encode_Fence.
+Require Import riscv.Proofs.invert_encode_R.
+Require Import riscv.Proofs.invert_encode_R_atomic.
+Require Import riscv.Proofs.invert_encode_I.
+Require Import riscv.Proofs.invert_encode_I_shift_57.
+Require Import riscv.Proofs.invert_encode_I_shift_66.
+Require Import riscv.Proofs.invert_encode_I_system.
+Require Import riscv.Proofs.invert_encode_S.
+Require Import riscv.Proofs.invert_encode_SB.
+Require Import riscv.Proofs.invert_encode_U.
+Require Import riscv.Proofs.invert_encode_UJ.
+Require Import riscv.Proofs.invert_encode_Fence.
 
 Local Open Scope bool_scope.
 Local Open Scope Z_scope.
@@ -39,29 +40,6 @@ Ltac somega_pre :=
 
 (* omega which understands bitSlice and shift *)
 Ltac somega := somega_pre; omega.
-
-Ltac write_as_pow2_opportunities f :=
-    repeat (so fun hyporgoal => match hyporgoal with
-               | context [ Z.pos ?p ] =>
-                   match p with
-                   | 1%positive => fail 1
-                   | 2%positive => fail 1
-                   | _ => idtac
-                   end;
-                   let e := eval cbv in (Z.log2 (Z.pos p)) in
-                   f (Z.pos p) (2 ^ e)
-               end);
-    (* we might have been a bit too eager -- undo undesired chained powers: *)
-    repeat (so fun hyporgoal => match hyporgoal with
-               | context [2 ^ 2 ^ ?p] => let r := eval cbv in (2 ^ p) in
-                                         change (2 ^ 2 ^ p) with (2 ^ r) in *
-               end).
-
-Tactic Notation "write_as_pow2" "in" "*|-" :=
-  write_as_pow2_opportunities ltac:(fun old new => change old with new in *|-).
-
-Tactic Notation "write_as_pow2" "in" "*" :=
-  write_as_pow2_opportunities ltac:(fun old new => change old with new in *).
 
 Lemma invert_encode_InvalidInstruction: forall i,
   verify_Invalid i ->
@@ -95,27 +73,20 @@ Ltac cbn_encode := repeat (
     opcode_BRANCH
     opcode_AUIPC
     opcode_AMO
-    funct3_JALR
     funct7_XOR
     funct7_SUBW
-    funct7_SRLIW
-    funct7_SRL
     funct7_SUB
     funct7_SRLW
+    funct7_SRLIW
+    funct7_SRL
+    funct7_SRAW
+    funct7_SRAIW
     funct7_SRA
     funct7_SLTU
     funct7_SLT
     funct7_SLLW
     funct7_SLLIW
     funct7_SLL
-    funct7_SRAW
-    funct7_SRAIW
-    funct7_MUL
-    funct7_DIVW
-    funct7_DIVUW
-    funct7_DIVU
-    funct7_DIV
-    funct7_AND
     funct7_SFENCE_VMA
     funct7_REMW
     funct7_REMUW
@@ -126,12 +97,25 @@ Ltac cbn_encode := repeat (
     funct7_MULHU
     funct7_MULHSU
     funct7_MULH
-    funct3_SRAIW
-    funct3_SRAI
-    funct3_SRA
-    funct3_SLTU
-    funct3_SLTIU
-    funct3_SLTI
+    funct7_MUL
+    funct7_FSUB_S
+    funct7_FSQRT_S
+    funct7_FSGNJ_S
+    funct7_FMV_X_W
+    funct7_FMV_W_X
+    funct7_FMUL_S
+    funct7_FMIN_S
+    funct7_FEQ_S
+    funct7_FDIV_S
+    funct7_FCVT_W_S
+    funct7_FCVT_S_W
+    funct7_FCLASS_S
+    funct7_FADD_S
+    funct7_DIVW
+    funct7_DIVUW
+    funct7_DIVU
+    funct7_DIV
+    funct7_AND
     funct7_ADDW
     funct7_ADD
     funct6_SRLI
@@ -158,8 +142,12 @@ Ltac cbn_encode := repeat (
     funct3_SRLI
     funct3_SRL
     funct3_SRAW
-    funct12_EBREAK
-    funct3_DIVUW
+    funct3_SRAIW
+    funct3_SRAI
+    funct3_SRA
+    funct3_SLTU
+    funct3_SLTIU
+    funct3_SLTI
     funct3_SLT
     funct3_SLLW
     funct3_SLLIW
@@ -187,10 +175,22 @@ Ltac cbn_encode := repeat (
     funct3_LD
     funct3_LBU
     funct3_LB
+    funct3_FSW
+    funct3_FSGNJ_S
+    funct3_FSGNJX_S
+    funct3_FSGNJN_S
+    funct3_FMV_X_W
+    funct3_FMIN_S
+    funct3_FMAX_S
+    funct3_FLW
+    funct3_FLT_S
+    funct3_FLE_S
+    funct3_FEQ_S
     funct3_FENCE_I
     funct3_FENCE
+    funct3_FCLASS_S
     funct3_DIVW
-    funct3_AND
+    funct3_DIVUW
     funct3_DIVU
     funct3_DIV
     funct3_CSRRWI
@@ -206,17 +206,20 @@ Ltac cbn_encode := repeat (
     funct3_BGE
     funct3_BEQ
     funct3_ANDI
-    funct12_URET
+    funct3_AND
     funct3_AMOW
     funct3_AMOD
     funct3_ADDW
     funct3_ADDIW
     funct3_ADDI
     funct3_ADD
+    funct2_FMADD_S
     funct12_WFI
-    funct12_MRET
+    funct12_URET
     funct12_SRET
+    funct12_MRET
     funct12_ECALL
+    funct12_EBREAK
     isValidM64
     isValidM
     isValidI64
@@ -224,31 +227,223 @@ Ltac cbn_encode := repeat (
     isValidCSR
     isValidA64
     isValidA
+    isValidF64
+    isValidF
     supportsM
     supportsA
+    supportsF
     bitwidth
     app
   ] in *;
   cbv [machineIntToShamt id] in *
 ).
 
-Lemma decode_encode: forall (inst: Instruction) (iset: InstructionSet),
-    verify inst iset ->
-    decode iset (encode inst) = inst.
-Proof.
-  intros. unfold verify in H. destruct H as [H H0].
-  unfold verify_iset in *.
-  cbv beta delta [decode].
+Ltac invert_encode_old :=
+  lazymatch goal with
+  | Henc: encode_I _ _ _ _ _ = _ |- _ =>
+    apply invert_encode_I in Henc
+  | Henc: encode_Fence _ _ _ _ _ _ _ = _ |- _ =>
+    apply invert_encode_Fence in Henc
+  | Henc: encode_I_shift_66 _ _ _ _ _ _ = _, iset: InstructionSet |- _ =>
+    apply (@invert_encode_I_shift_66 (bitwidth iset)) in Henc
+  | Henc: encode_I_shift_57 _ _ _ _ _ _ = _ |- _ =>
+    apply invert_encode_I_shift_57 in Henc
+  | Henc: encode_R _ _ _ _ _ _ = _ |- _ =>
+    apply invert_encode_R in Henc
+  | Henc: encode_Invalid _ = _ |- _ =>
+    apply invert_encode_InvalidInstruction in Henc; case Henc
+  | Henc: encode_R_atomic _ _ _ _ _ _ _ = _ |- _ =>
+    apply invert_encode_R_atomic in Henc
+  | Henc: encode_I_system _ _ _ _ _ = _ |- _ =>
+    apply invert_encode_I_system in Henc
+  | Henc: encode_U _ _ _ = _ |- _ =>
+    apply invert_encode_U in Henc
+  | Henc: encode_UJ _ _ _ = _ |- _ =>
+    apply invert_encode_UJ in Henc
+  | Henc: encode_S _ _ _ _ _ = _ |- _ =>
+    apply invert_encode_S in Henc
+  | Henc: encode_SB _ _ _ _ _ = _ |- _ =>
+    apply invert_encode_SB in Henc
+  end;
+  [|assumption..].
+
+(* requires iset to be destructed *)
+Ltac simpl_results_list :=
+  cbv beta iota delta [
+    isValidM64
+    isValidM
+    isValidI64
+    isValidI
+    isValidCSR
+    isValidA64
+    isValidA
+    isValidF64
+    isValidF
+    supportsM
+    supportsA
+    supportsF
+    bitwidth
+  ] in *;
+  change (32 =? 64) with false in *;
+  change (64 =? 64) with true in *;
+  change (true && false) with false in *;
+  change (true && true) with true in *;
+  change (false && false) with false in *;
+  change (false && true) with false in *;
+  cbv iota in *.
+
+Set Printing Depth 1000000.
+
+Ltac define_decoder :=
+  let x := fresh "x" in let iset := fresh "iset" in let inst := fresh "inst" in
+  intros iset inst;
+  set (x := decode iset inst);
+  revert x;
+  cbv beta delta [decode];
   repeat match goal with
-  | |- (let x := ?a in ?b) = ?c => change (let x := a in b = c); intro
-  | x := ?t : ?T |- _ => pose proof (eq_refl t : x = t); clearbody x
+  | |- let x := let y := ?A in (@?B y) in ?C =>
+    set (y := A); change (let x := (B y) in C); cbv beta
+  end;
+  intro x.
+
+
+Definition mdecodeI': InstructionSet -> MachineInt -> InstructionI.
+  define_decoder. exact decodeI.
+Defined.
+Definition mdecodeI: InstructionSet -> MachineInt -> InstructionI :=
+  Eval cbv [decode mdecodeI'] in mdecodeI'.
+
+Definition mdecodeM': InstructionSet -> MachineInt -> InstructionM.
+  define_decoder. exact decodeM.
+Defined.
+Definition mdecodeM: InstructionSet -> MachineInt -> InstructionM :=
+  Eval cbv [decode mdecodeM'] in mdecodeM'.
+
+Definition mdecodeA': InstructionSet -> MachineInt -> InstructionA.
+  define_decoder. exact decodeA.
+Defined.
+Definition mdecodeA: InstructionSet -> MachineInt -> InstructionA :=
+  Eval cbv [decode mdecodeA'] in mdecodeA'.
+
+Definition mdecodeF': InstructionSet -> MachineInt -> InstructionF.
+  define_decoder. exact decodeF.
+Defined.
+Definition mdecodeF: InstructionSet -> MachineInt -> InstructionF :=
+  Eval cbv [decode mdecodeF'] in mdecodeF'.
+
+Definition mdecodeI64': InstructionSet -> MachineInt -> InstructionI64.
+  define_decoder. exact decodeI64.
+Defined.
+Definition mdecodeI64: InstructionSet -> MachineInt -> InstructionI64 :=
+  Eval cbv [decode mdecodeI64'] in mdecodeI64'.
+
+Definition mdecodeM64': InstructionSet -> MachineInt -> InstructionM64.
+  define_decoder. exact decodeM64.
+Defined.
+Definition mdecodeM64: InstructionSet -> MachineInt -> InstructionM64 :=
+  Eval cbv [decode mdecodeM64'] in mdecodeM64'.
+
+Definition mdecodeA64': InstructionSet -> MachineInt -> InstructionA64.
+  define_decoder. exact decodeA64.
+Defined.
+Definition mdecodeA64: InstructionSet -> MachineInt -> InstructionA64 :=
+  Eval cbv [decode mdecodeA64'] in mdecodeA64'.
+
+Definition mdecodeF64': InstructionSet -> MachineInt -> InstructionF64.
+  define_decoder. exact decodeF64.
+Defined.
+Definition mdecodeF64: InstructionSet -> MachineInt -> InstructionF64 :=
+  Eval cbv [decode mdecodeF64'] in mdecodeF64'.
+
+Definition mdecodeCSR': InstructionSet -> MachineInt -> InstructionCSR.
+  define_decoder. exact decodeCSR.
+Defined.
+Definition mdecodeCSR: InstructionSet -> MachineInt -> InstructionCSR :=
+  Eval cbv [decode mdecodeCSR'] in mdecodeCSR'.
+
+Definition modular_decode': InstructionSet -> MachineInt -> Instruction.
+  define_decoder.
+  change decodeI with (mdecodeI iset inst) in *; clear decodeI.
+  change decodeM with (mdecodeM iset inst) in *; clear decodeM.
+  change decodeA with (mdecodeA iset inst) in *; clear decodeA.
+  change decodeF with (mdecodeF iset inst) in *; clear decodeF.
+  change decodeI64 with (mdecodeI64 iset inst) in *; clear decodeI64.
+  change decodeM64 with (mdecodeM64 iset inst) in *; clear decodeM64.
+  change decodeA64 with (mdecodeA64 iset inst) in *; clear decodeA64.
+  change decodeF64 with (mdecodeF64 iset inst) in *; clear decodeF64.
+  change decodeCSR with (mdecodeCSR iset inst) in *; clear decodeCSR.
+  clear -x.
+  (* almost copy-pastable *)
+Abort.
+
+Definition modular_decode(iset: InstructionSet)(inst: MachineInt): Instruction :=
+  let resultCSR := if isValidCSR (mdecodeCSR iset inst)
+                   then [CSRInstruction (mdecodeCSR iset inst)]
+                   else [] in
+  let resultF64 := if isValidF64 (mdecodeF64 iset inst)
+                   then [F64Instruction (mdecodeF64 iset inst)]
+                   else [] in
+  let resultA64 := if isValidA64 (mdecodeA64 iset inst)
+                   then [A64Instruction (mdecodeA64 iset inst)]
+                   else [] in
+  let resultM64 := if isValidM64 (mdecodeM64 iset inst)
+                   then [M64Instruction (mdecodeM64 iset inst)]
+                   else [] in
+  let resultI64 := if isValidI64 (mdecodeI64 iset inst)
+                   then [I64Instruction (mdecodeI64 iset inst)]
+                   else [] in
+  let resultF := if isValidF (mdecodeF iset inst) then [FInstruction (mdecodeF iset inst)] else [] in
+  let resultA := if isValidA (mdecodeA iset inst) then [AInstruction (mdecodeA iset inst)] else [] in
+  let resultM := if isValidM (mdecodeM iset inst) then [MInstruction (mdecodeM iset inst)] else [] in
+  let resultI := if isValidI (mdecodeI iset inst) then [IInstruction (mdecodeI iset inst)] else [] in
+  let results := resultI ++
+                 (if supportsM iset then resultM else []) ++
+                 (if supportsA iset then resultA else []) ++
+                 (if supportsF iset then resultF else []) ++
+                 (if bitwidth iset =? 64 then resultI64 else []) ++
+                 (if (bitwidth iset =? 64) && supportsM iset then resultM64 else []) ++
+                 (if (bitwidth iset =? 64) && supportsA iset then resultA64 else []) ++
+                 (if (bitwidth iset =? 64) && supportsF iset then resultF64 else []) ++
+                 resultCSR in
+           if BinInt.Z.of_nat (length results) >? 1
+           then InvalidInstruction inst
+           else nth 0 results (InvalidInstruction inst).
+
+Lemma decode_alt: forall iset inst, decode iset inst = modular_decode iset inst.
+Proof.
+  intros. reflexivity.
+Qed.
+
+Ltac invert_encode :=
+  match goal with
+  | E: _, V: _ |- _ => case (invert_encode_InvalidInstruction _ V _ E)
+  | E: _, V: _ |- _ => pose proof (invert_encode_I V _ E); clear E V
+  | E: _, V: _ |- _ => pose proof (invert_encode_Fence V _ E); clear E V
+  | E: _, V: _ |- _ => pose proof (invert_encode_I_shift_66 V _ E); clear E V
+  | E: _, V: _ |- _ => pose proof (invert_encode_I_shift_57 V _ E); clear E V
+  | E: _, V: _ |- _ => pose proof (invert_encode_R V _ E); clear E V
+  | E: _, V: _ |- _ => pose proof (invert_encode_R_atomic V _ E); clear E V
+  | E: _, V: _ |- _ => pose proof (invert_encode_I_system V _ E); clear E V
+  | E: _, V: _ |- _ => pose proof (invert_encode_U V _ E); clear E V
+  | E: _, V: _ |- _ => pose proof (invert_encode_UJ V _ E); clear E V
+  | E: _, V: _ |- _ => pose proof (invert_encode_S V _ E); clear E V
+  | E: _, V: _ |- _ => pose proof (invert_encode_SB V _ E); clear E V
   end.
-  remember (encode inst) as encoded eqn:Henc; symmetry in Henc.
-  cbv [encode] in Henc.
+
+Ltac prove_decode_encode :=
+  let iset := fresh "iset" in let inst := fresh "inst" in let V := fresh "V" in
+  intros iset inst V; unfold verify in V; destruct V;
+  unfold verify_iset in *;
+  let Henc := fresh "Henc" in
+  match goal with
+  | |- ?D ?I (encode ?x) = _ =>
+    remember (encode x) as encoded eqn:Henc; symmetry in Henc
+  end;
+  cbv [encode] in Henc;
   cbv [
       Encoder
         Verifier
-        apply_InstructionMapper 
+        apply_InstructionMapper
         map_Fence
         map_I
         map_I_shift_57
@@ -261,54 +456,35 @@ Proof.
         map_SB
         map_U
         map_UJ
-    ] in Henc.
-
-  destruct inst as [i|i|i|i|i|i|i|i].
-  par: abstract (destruct i; try (
-    (lazymatch type of Henc with
-     | encode_I _ _ _ _ _ = _ =>
-       apply invert_encode_I in Henc
-     | encode_Fence _ _ _ _ _ _ _ = _ =>
-       apply invert_encode_Fence in Henc
-     | encode_I_shift_66 _ _ _ _ _ _ = _ =>
-       apply (@invert_encode_I_shift_66 (bitwidth iset)) in Henc
-     | encode_I_shift_57 _ _ _ _ _ _ = _ =>
-       apply invert_encode_I_shift_57 in Henc
-     | encode_R _ _ _ _ _ _ = _ =>
-       apply invert_encode_R in Henc
-     | encode_Invalid _ = _ =>
-       apply invert_encode_InvalidInstruction in Henc
-     | encode_R_atomic _ _ _ _ _ _ _ = _ => 
-       apply invert_encode_R_atomic in Henc
-     | encode_I_system _ _ _ _ _ = _ =>
-       apply invert_encode_I_system in Henc
-     | encode_U _ _ _ = _ =>
-       apply invert_encode_U in Henc
-     | encode_UJ _ _ _ = _ =>
-       apply invert_encode_UJ in Henc
-     | encode_S _ _ _ _ _ = _ =>
-       apply invert_encode_S in Henc
-     | encode_SB _ _ _ _ _ = _ => 
-       apply invert_encode_SB in Henc
-     end; [|trivial]);
+    ] in Henc;
+  match goal with
+  | |- ?D ?I _ = _ => cbv [D]
+  end;
+  (* will split from 1 goal into ~8 goals *)
+  destruct iset;
+  try abstract (
+    (* multiplies number of goals by up to 80 *)
+    destruct inst;
+    invert_encode;
+    match goal with
+    | Henc: _ /\ _ |- _ =>
       repeat match type of Henc with
-               _ /\ _ => let H := fresh "H" in destruct Henc as [H Henc]; rewrite <-?H in *
-             end; rewrite <-?Henc in *;
-      subst results; subst resultI; subst decodeI; subst opcode; subst funct3;
-      subst funct5; subst funct6; subst funct7; subst funct10; subst funct12;
-      destruct iset;
-      repeat match goal with
-      | H: False |- _ => destruct H
-      | |- ?x = ?x => exact_no_check (eq_refl x)
-      | |- _ => progress cbn_encode
-      | |- _ => rewrite !Bool.orb_true_r in *
-      | |- _ => rewrite !Bool.andb_false_r in *
-      | |- _ => progress subst
-      end);
-     (* cases where bitSlice in goal and hyps do not match *)
-     cbv [funct7_SFENCE_VMA opcode_SYSTEM funct3_PRIV funct12_WFI funct12_MRET
-          funct12_SRET funct12_URET funct12_EBREAK funct12_ECALL
-          funct3_FENCE_I opcode_MISC_MEM isValidI] in *;
+             |  _ /\ _ => let H := fresh "H" in destruct Henc as [H Henc]; rewrite <-?H in *
+             end;
+        rewrite <-?Henc in *
+    end;
+    repeat match goal with
+    | |- (if ?b then ?x else ?y) = ?z => change (y = z)
+    end;
+    match goal with
+    | |- (if ?b then ?x else ?y) = ?z => change (x = z); reflexivity
+    | |- (if ?b then ?x else ?y) = ?x => replace b with true; [reflexivity|]
+    end;
+    (* cases where bitSlice in goal and hyps do not match *)
+    repeat match goal with
+           | |- context [?a =?  _] => unfold a
+           | |- context [_  =? ?a] => unfold a
+           end;
      repeat match goal with
             | |- ?x = ?x => exact_no_check (eq_refl x)
             | |- context [?x =? ?y] =>
@@ -321,6 +497,87 @@ Proof.
      try solve [ exfalso;
                  try (match goal with H: _ <> _ |- _ => apply H; clear H end);
                  somega ]).
+
+Lemma mdecodeI_encode: forall (inst: InstructionI) (iset: InstructionSet),
+    verify (IInstruction inst) iset ->
+    mdecodeI iset (encode (IInstruction inst)) = inst.
+Proof.
+  prove_decode_encode.
 Qed.
 
-Print Assumptions decode_encode.
+Lemma mdecodeM_encode: forall (inst: InstructionM) (iset: InstructionSet),
+    verify (MInstruction inst) iset ->
+    mdecodeM iset (encode (MInstruction inst)) = inst.
+Proof.
+  prove_decode_encode.
+Qed.
+
+Lemma mdecodeA_encode: forall (inst: InstructionA) (iset: InstructionSet),
+    verify (AInstruction inst) iset ->
+    mdecodeA iset (encode (AInstruction inst)) = inst.
+Proof.
+  prove_decode_encode.
+Qed.
+
+Lemma mdecodeF_encode: forall (inst: InstructionF) (iset: InstructionSet),
+    verify (FInstruction inst) iset ->
+    mdecodeF iset (encode (FInstruction inst)) = inst.
+Proof.
+  prove_decode_encode.
+Qed.
+
+Lemma mdecodeI64_encode: forall (inst: InstructionI64) (iset: InstructionSet),
+    verify (I64Instruction inst) iset ->
+    mdecodeI64 iset (encode (I64Instruction inst)) = inst.
+Proof.
+  prove_decode_encode.
+Qed.
+
+Lemma mdecodeM64_encode: forall (inst: InstructionM64) (iset: InstructionSet),
+    verify (M64Instruction inst) iset ->
+    mdecodeM64 iset (encode (M64Instruction inst)) = inst.
+Proof.
+  prove_decode_encode.
+Qed.
+
+Lemma mdecodeA64_encode: forall (inst: InstructionA64) (iset: InstructionSet),
+    verify (A64Instruction inst) iset ->
+    mdecodeA64 iset (encode (A64Instruction inst)) = inst.
+Proof.
+  prove_decode_encode.
+Qed.
+
+Lemma mdecodeF64_encode: forall (inst: InstructionF64) (iset: InstructionSet),
+    verify (F64Instruction inst) iset ->
+    mdecodeF64 iset (encode (F64Instruction inst)) = inst.
+Proof.
+  prove_decode_encode.
+Qed.
+
+Lemma mdecodeCSR_encode: forall (inst: InstructionCSR) (iset: InstructionSet),
+    verify (CSRInstruction inst) iset ->
+    mdecodeCSR iset (encode (CSRInstruction inst)) = inst.
+Proof.
+  (* prove_decode_encode. *)
+  (* TODO inst/iset swapped! *)
+Admitted.
+
+Lemma mdecodeM_I: forall inst iset,
+    mdecodeM iset (encode (IInstruction inst)) = InvalidM.
+Proof.
+  intros. cbv beta delta [mdecodeM].
+  (* bad idea: requires us to do the whole case splitting again *)
+Abort.
+
+Lemma decode_encode: forall (inst: Instruction) (iset: InstructionSet),
+    verify inst iset ->
+    decode iset (encode inst) = inst.
+Proof.
+  destruct inst; intros.
+  - apply mdecodeI_encode in H.
+    rewrite decode_alt.
+    cbv beta delta [modular_decode].
+    rewrite H.
+    simpl.
+    (* not sure if the "modular" approach pays off *)
+Admitted.
